examples/graph/lib/Data/Graph/Inductive/Query/BFS.v
@@ -26,6 +26,13 @@ Import GHC.Num.Notations.
 
 (* No type declarations to convert. *)
 
+(* Midamble *)
+
+Instance LPath__Default {a} : GHC.Err.Default (Data.Graph.Inductive.Graph.LPath a) :=
+  { default := Data.Graph.Inductive.Graph.LP nil }.
+
+Instance Queue__Default {a} : GHC.Err.Default (Data.Graph.Inductive.Internal.Queue.Queue a) :=
+  { default := Data.Graph.Inductive.Internal.Queue.MkQueue nil nil }.
 (* Converted value declarations: *)
 
 Definition suci {a} {b}
