examples/graph/module-edits/Data/Graph/Inductive/Internal/Heap/preamble.v
@@ -1,1 +1,3 @@
 Require Import Coq.Lists.List.
+Require Import Omega.
+Require Import Wellfounded.
