examples/graph/module-edits/Data/Graph/Inductive/Query/BFS/midamble.v
@@ -1,0 +1,5 @@
+Instance LPath__Default {a} : GHC.Err.Default (Data.Graph.Inductive.Graph.LPath a) :=
+  { default := Data.Graph.Inductive.Graph.LP nil }.
+
+Instance Queue__Default {a} : GHC.Err.Default (Data.Graph.Inductive.Internal.Queue.Queue a) :=
+  { default := Data.Graph.Inductive.Internal.Queue.MkQueue nil nil }.
